theories/Lambda/ExprCore.v
@@ -21,28 +21,42 @@ Section env.
   | Inj : func -> expr
   | App : expr -> expr -> expr
   | Abs : typ -> expr -> expr
-  | UVar : uvar -> expr.
+  | UVar : uvar -> list expr -> expr.
 
   Inductive expr_acc : expr -> expr -> Prop :=
   | acc_App_l : forall f a, expr_acc f (App f a)
   | acc_App_r : forall f a, expr_acc a (App f a)
-  | acc_Abs : forall t e, expr_acc e (Abs t e).
+  | acc_Abs : forall t e, expr_acc e (Abs t e)
+  | acc_UVar : forall u es e, In e es -> expr_acc e (UVar u es).
 
   Definition exprs : Type := list expr.
 
   Theorem wf_expr_acc : well_founded expr_acc.
   Proof.
     clear. red.
-    induction a; simpl; intros; constructor; intros;
+(*    refine (fix recurse a : Acc expr_acc a :=
+              match a as a return Acc expr_acc a with
+                | Var v => Acc_intro _ (fun y pf => match pf in expr_acc _ z return match z return Prop with
+                                                                                      | Var v => Acc expr_acc y
+                                                                                      | _ => True
+                                                                                    end
+                                                    with
+                                                      | acc_App_l _ _ => _
+                                                      | _ => _
+                                                    end)
+                | App f x => _
+                | _ => _
+              end) ;
     try solve [ inversion H ].
-    { inversion H; clear H; subst; auto. }
-    { inversion H; clear H; subst; auto. }
-  Defined.
+constructor.
+Show Proof.
+*)
+  Admitted.
 
   Theorem expr_strong_ind
   : forall (P : expr -> Prop),
       (forall v, P (Var v)) ->
-      (forall u, P (UVar u)) ->
+      (forall u es, Forall P es -> P (UVar u es)) ->
       (forall i, P (Inj i)) ->
       (forall a b, (forall e, (leftTrans expr_acc) e (App a b) -> P e) -> P (App a b)) ->
       (forall t a, (forall e, (leftTrans expr_acc) e (Abs t a) -> P e) -> P (Abs t a)) ->
@@ -51,6 +65,7 @@ Section env.
     intros P Hvar Huvar Hinj Happ Habs.
     eapply Fix. eapply wf_leftTrans. eapply wf_expr_acc.
     destruct x; auto.
+    intros. eapply Huvar. clear - H. admit.
   Qed.
 
   Variable RelDec_eq_typ : RelDec (@eq typ).
@@ -61,7 +76,16 @@ Section env.
   Fixpoint expr_eq_dec (e1 e2 : expr) : bool :=
     match e1 , e2 with
       | Var v1 , Var v2 => EqNat.beq_nat v1 v2
-      | UVar v1 , UVar v2 => EqNat.beq_nat v1 v2
+      | UVar v1 es1 , UVar v2 es2 =>
+        if EqNat.beq_nat v1 v2 then
+          (fix go a b : bool :=
+             match a , b with
+               | nil , nil => true
+               | x :: xs , y :: ys => expr_eq_dec x y && go xs ys
+               | _ , _ => false
+             end)
+            es1 es2
+        else false
       | Inj f1 , Inj f2 =>
         f1 ?[ eq ] f2
       | App f1 e1 , App f2 e2 =>
@@ -99,6 +123,7 @@ Section env.
              | |- _ => rewrite andb_true_iff
              | H : forall x, (_ = true) <-> _ |- _ => rewrite H
            end; try solve [ intuition congruence ].
+    admit.
   Qed.
 
   Global Instance RelDec_eq_expr : RelDec (@eq expr) :=
@@ -116,7 +141,9 @@ Section env.
       match e with
         | Var _
         | Inj _ => false
-        | UVar u' => EqNat.beq_nat u u'
+        | UVar u' us =>
+          if EqNat.beq_nat u u' then true
+          else List.existsb mentionsU us
         | App f e => if mentionsU f then true else mentionsU e
         | Abs _ e => mentionsU e
       end.
@@ -126,8 +153,8 @@ Section env.
     Fixpoint mentionsV (v : var) (e : expr) : bool :=
       match e with
         | Var v' => v ?[ eq ] v'
-        | Inj _
-        | UVar _ => false
+        | Inj _ => false
+        | UVar _ us => List.existsb (mentionsV v) us
         | App a b => if mentionsV v a then true else mentionsV v b
         | Abs _ e => mentionsV (S v) e
       end.
@@ -137,7 +164,7 @@ End env.
 
 Arguments Var {typ func} _.
 Arguments Inj {typ func} _.
-Arguments UVar {typ func} _.
+Arguments UVar {typ func} _ _.
 Arguments App {typ func} _ _.
 Arguments Abs {typ func} _ _.
 Arguments mentionsU {typ func} _ _.
