theories/EnvI.v
@@ -10,41 +10,22 @@ Set Strict Implicit.
 
 Section Env.
   Variable typ : Type.
-  Context {RType_typ : RType typ}.
+  Variable denote : typ -> Type.
 
   (** Environments **)
   Definition tenv : Type := list typ.
-  Definition env : Type := list (sigT (@typD _ _)).
+  Definition env : Type := list (sigT denote).
 
   Definition typeof_env (e : env) : tenv :=
     map (@projT1 _ _) e.
 
-  Definition lookupAs (e : env) (n : nat) (ty : typ) : option (typD ty) :=
-    match nth_error e n with
-      | None => None
-      | Some (existT t v) =>
-        match type_cast ty t with
-          | Some pf => Some (Relim (fun x => x) pf v)
-          | None => None
-        end
-    end.
-
-  Theorem lookupAs_weaken : forall (a b : env) n t x,
-    lookupAs a n t = Some x ->
-    lookupAs (a ++ b) n t = Some x.
-  Proof.
-    clear. unfold lookupAs. intros.
-    consider (nth_error a n); intros; try congruence.
-    erewrite nth_error_weaken by eassumption. auto.
-  Qed.
-
-  Fixpoint join_env (gs : list typ) (hgs : hlist (@typD _ _) gs) : env :=
+  Fixpoint join_env (gs : list typ) (hgs : hlist denote gs) : env :=
     match hgs with
       | Hnil => nil
       | Hcons a b c d => existT _ _ c :: join_env d
     end.
 
-  Fixpoint split_env (gs : env) : sigT (hlist (@typD _ _)) :=
+  Fixpoint split_env (gs : env) : sigT (hlist denote) :=
     match gs with
       | nil => existT _ nil Hnil
       | g :: gs =>
@@ -91,7 +72,7 @@ Section Env.
     nth_error ve v = Some tv <->
     match nth_error (projT1 (split_env ve)) v as t
           return match t with
-                   | Some v => typD v
+                   | Some v => denote v
                    | None => unit
                  end -> Prop
     with
@@ -327,6 +308,6 @@ Section nth_error_get_hlist_nth.
 
 End nth_error_get_hlist_nth.
 
-Arguments env {typ _} : rename.
+Arguments env {typ} _ : rename.
 Arguments join_env {typ _ _} _ : rename.
 Arguments split_env {typ _} _ : rename.
