theories/InstantiateI.v
@@ -4,6 +4,24 @@ Require Import MirrorCore.EnvI.
 Require Import MirrorCore.ExprI.
 Require Import MirrorCore.TypesI.
 
+Fixpoint hlist_build {T U} (F : T -> Type) (f : forall x : T, U -> option (F x))
+           (ls : list T) (ls' : list U)
+: option (hlist F ls) :=
+  match ls as ls , ls' return option (hlist F ls) with
+    | nil , nil => Some Hnil
+    | l :: ls , l' :: ls' =>
+      match hlist_build F f ls ls' with
+        | None => None
+        | Some res =>
+          match f l l' with
+            | None => None
+            | Some x =>
+              Some (Hcons x res)
+          end
+      end
+    | _ , _ => None
+  end.
+
 Section definitions.
   Variables typ expr : Type.
   Context {RType_typ : RType typ}.
@@ -11,20 +29,24 @@ Section definitions.
   Context {ExprOk_expr : ExprOk Expr_expr}.
 
   (** instantiate **)
-  Variable instantiate : (nat -> option expr) -> nat -> expr -> expr.
+  Variable instantiate : (nat -> list expr -> option expr) -> nat -> expr -> expr.
 
-  Definition sem_preserves_if tus tvs
-             (P : hlist _ tus -> hlist _ tvs -> Prop)
-             (f : nat -> option expr) : Prop :=
-    forall u e t get,
-      f u = Some e ->
+  Definition sem_preserves_if (tus : tenv (tenv typ * typ)) (tvs : tenv typ)
+             (P : OpenT tus tvs Prop)
+             (f : nat -> list expr -> option expr) : Prop :=
+    forall u e es t get vals,
+      f u es = Some e ->
       nth_error_get_hlist_nth _ tus u = Some (@existT _ _ t get) ->
+      hlist_build (fun T => OpenT tus tvs (typD T))
+                  (fun t e => exprD' tus tvs e t) (fst t) es = Some vals ->
       exists eD,
-        exprD' tus tvs e t = Some eD /\
+        exprD' tus tvs e (snd t) = Some eD /\
         forall us vs,
           P us vs ->
-          get us = eD us vs.
+          get us (hlist_map (fun t (x : OpenT tus tvs (typD t)) => x us vs) vals) = eD us vs.
 
+  (** TODO **)
+(*
   Definition instantiate_mentionsU : Prop :=
     forall f n e u,
       mentionsU u (instantiate f n e) = true <-> (** do i need iff? **)
@@ -33,6 +55,7 @@ Section definitions.
             f u' = Some e' /\
             mentionsU u' e = true/\
             mentionsU u e' = true).
+*)
 
   Definition exprD'_instantiate : Prop :=
     forall tus tvs f e tvs' t eD P,
